add LO.Logic

Logic/Logic/System.lean
@@ -1,4 +1,4 @@
-import Logic.Logic.LogicSymbol
+import Logic.Logic.Semantics
 
 namespace LO
 
@@ -47,73 +47,6 @@ def System.hom [System F] {G : Type u} [LogicSymbol G] (F : G →L F) : System G
   axm := fun h => System.axm (Set.mem_image_of_mem F h)
   weakening' := fun h => by simp; exact System.weakening' (Set.image_subset F h)
 
-/- Semantics of F -/
-
-class Semantics (F : Type u) [LogicSymbol F] (Struc : outParam (Type w → Type v)) where
-  models : {M : Type w} → Struc M → F →L Prop
-
-namespace Semantics
-variable {Struc : Type w → Type v} [𝓢 : Semantics F Struc]
-
-def modelsTheory {M : Type w} (s : Struc M) (T : Set F) : Prop :=
-    ∀ ⦃f⦄, f ∈ T → models s f
-
-postfix:max " ⊧ₛ " => models
-
-infix:55 " ⊧ₛ* " => modelsTheory
-
-def consequence (T : Set F) (f : F) : Prop :=
-    ∀ (M : Type w) [Inhabited M] (s : Struc M), s ⊧ₛ* T → s ⊧ₛ f
-
--- note that ⊨ (\vDash) is *NOT* ⊧ (\models)
-infix:55 " ⊨ " => consequence
-
-def Valid (f : F) : Prop := ∀ ⦃M : Type w⦄ [Inhabited M] (s : Struc M), s ⊧ₛ f
-
-def Validₛ (T : Set F) : Prop := ∀ ⦃M : Type w⦄ [Inhabited M] (s : Struc M), s ⊧ₛ* T
-
-def Satisfiable (f : F) : Prop := ∃ (M : Type w) (_ : Inhabited M) (s : Struc M), s ⊧ₛ f
-
-def Satisfiableₛ (T : Set F) : Prop := ∃ (M : Type w) (_ : Inhabited M) (s : Struc M), s ⊧ₛ* T
-
-lemma valid_neg_iff (f : F) : Valid (~f) ↔ ¬Satisfiable f := by simp[Valid, Satisfiable]
-
-lemma not_satisfiable_finset [DecidableEq F] (t : Finset F) :
-    ¬Satisfiableₛ (t : Set F) ↔ Valid (t.image (~·)).disj :=
-  by simp[Satisfiableₛ, modelsTheory, Valid, Finset.map_disj]
-
-lemma modelsTheory_of_subset {T U : Set F} {s : Struc M} (h : s ⊧ₛ* U) (ss : T ⊆ U) : s ⊧ₛ* T :=
-  fun _ hf => h (ss hf)
-
-@[simp] lemma modelsTheoryEmpty {s : Struc M} : s ⊧ₛ* (∅ : Set F) := fun p => by simp
-
-@[simp] lemma modelsTheory_insert {T : Set F} {f : F} {s : Struc M} :
-    s ⊧ₛ* insert f T ↔ s ⊧ₛ f ∧ s ⊧ₛ* T := by
-  simp[modelsTheory]
-
-@[simp] lemma modelsTheory_union {T U : Set F} {s : Struc M} :
-    s ⊧ₛ* T ∪ U ↔ s ⊧ₛ* T ∧ s ⊧ₛ* U := by
-  simp[modelsTheory]
-  exact
-  ⟨fun h => ⟨fun f hf => h (Or.inl hf), fun f hf => h (Or.inr hf)⟩,
-   by rintro ⟨h₁, h₂⟩ f (h | h); exact h₁ h; exact h₂ h⟩
-
-@[simp] lemma modelsTheory_image {f : α → F} {A : Set α} {s : Struc M} :
-    s ⊧ₛ* f '' A ↔ ∀ i ∈ A, s ⊧ₛ (f i) := by simp[modelsTheory]
-
-@[simp] lemma modelsTheory_range {f : α → F} {s : Struc M} :
-    s ⊧ₛ* Set.range f ↔ ∀ i, s ⊧ₛ (f i) := by simp[modelsTheory]
-
-lemma satisfiableₛ_of_subset {T U : Set F} (h : Satisfiableₛ U) (ss : T ⊆ U) : Satisfiableₛ T :=
-  by rcases h with ⟨M, i, s, h⟩; exact ⟨M, i, s, modelsTheory_of_subset h ss⟩
-
-lemma consequence_iff {T : Set F} {f : F} : T ⊨ f ↔ ¬Satisfiableₛ (insert (~f) T) := by
-  simp[consequence, Satisfiableₛ]; constructor
-  · intro h M hM s hf hT; have : s ⊧ₛ f := h M s hT; contradiction
-  · intro h M hM s; contrapose; exact h M hM s
-
-end Semantics
-
 variable (F)
 variable [LogicSymbol F] [𝓑 : System F] {Struc : Type w → Type v} [𝓢 : Semantics F Struc]
 
@@ -122,9 +55,6 @@ class Sound where
 
 class SoundOn (M : Type w) (s : Struc M) (H : Set F) where
   sound : ∀ {T : Set F} {p : F}, p ∈ H → T ⊢ p → s ⊧ₛ p
-
-class Compact where
-  compact {T : Set F} : Semantics.Satisfiableₛ T ↔ (∀ u : Finset F, (u : Set F) ⊆ T → Semantics.Satisfiableₛ (u : Set F))
 
 class Complete extends Sound F where
   complete : ∀ {T : Set F} {p : F}, T ⊨ p → T ⊢ p
@@ -154,20 +84,6 @@ lemma modelsTheory_of_proofTheory {T U : Set F} (h : s ⊧ₛ* T) (b : T ⊢* U)
   fun _ hf => models_of_proof h (b hf)
 
 end Sound
-
-namespace Compact
-
-variable [Compact F]
-variable {M : Type w} [Inhabited M] {s : Struc M}
-
-lemma conseq_compact [DecidableEq F] {f : F} :
-    T ⊨ f ↔ ∃ u : Finset F, ↑u ⊆ T ∧ u ⊨ f := by
-  simp[Semantics.consequence_iff, compact (T := insert (~f) T)]
-  constructor
-  · intro ⟨u, ss, hu⟩; exact ⟨Finset.erase u (~f), by simp[ss], by { simp; intro h; exact hu (Semantics.satisfiableₛ_of_subset h (by simp)) }⟩
-  · intro ⟨u, ss, hu⟩; exact ⟨insert (~f) u, by simpa using Set.insert_subset_insert ss, by simpa using hu⟩
-
-end Compact
 
 namespace Complete
 
