Logic/Logic/Semantics.lean
@@ -1,0 +1,106 @@
+import Logic.Logic.LogicSymbol
+
+namespace LO
+
+variable {F : Type u} [LogicSymbol F]
+
+class Semantics (F : Type u) [LogicSymbol F] (Struc : outParam (Type w → Type v)) where
+  models : {M : Type w} → Struc M → F →L Prop
+
+class Vocabulary (F : Type u) [LogicSymbol F] (V : outParam (Type v)) where
+  voc    : F → Set V
+  verum  : voc ⊤ = ∅
+  falsum : voc ⊥ = ∅
+  neg    : (f : F) → voc (~f) = voc f
+  and    : (f g : F) → voc (f ⋏ g) = voc f ∪ voc g
+  or     : (f g : F) → voc (f ⋎ g) = voc f ∪ voc g
+  imp    : (f g : F) → voc (f ⟶ g) = voc f ∪ voc g
+
+class Logic (F : Type u) [LogicSymbol F] (Struc : outParam (Type w → Type v)) (V : outParam (Type v'))
+  extends Semantics F Struc, Vocabulary F V
+
+namespace Semantics
+variable {Struc : Type w → Type v} [𝓢 : Semantics F Struc]
+
+def modelsTheory {M : Type w} (s : Struc M) (T : Set F) : Prop :=
+    ∀ ⦃f⦄, f ∈ T → models s f
+
+postfix:max " ⊧ₛ " => models
+
+infix:55 " ⊧ₛ* " => modelsTheory
+
+def consequence (T : Set F) (f : F) : Prop :=
+    ∀ (M : Type w) [Inhabited M] (s : Struc M), s ⊧ₛ* T → s ⊧ₛ f
+
+-- note that ⊨ (\vDash) is *NOT* ⊧ (\models)
+infix:55 " ⊨ " => consequence
+
+def Valid (f : F) : Prop := ∀ ⦃M : Type w⦄ [Inhabited M] (s : Struc M), s ⊧ₛ f
+
+def Validₛ (T : Set F) : Prop := ∀ ⦃M : Type w⦄ [Inhabited M] (s : Struc M), s ⊧ₛ* T
+
+def Satisfiable (f : F) : Prop := ∃ (M : Type w) (_ : Inhabited M) (s : Struc M), s ⊧ₛ f
+
+def Satisfiableₛ (T : Set F) : Prop := ∃ (M : Type w) (_ : Inhabited M) (s : Struc M), s ⊧ₛ* T
+
+lemma valid_neg_iff (f : F) : Valid (~f) ↔ ¬Satisfiable f := by simp[Valid, Satisfiable]
+
+lemma not_satisfiable_finset [DecidableEq F] (t : Finset F) :
+    ¬Satisfiableₛ (t : Set F) ↔ Valid (t.image (~·)).disj :=
+  by simp[Satisfiableₛ, modelsTheory, Valid, Finset.map_disj]
+
+lemma modelsTheory_of_subset {T U : Set F} {s : Struc M} (h : s ⊧ₛ* U) (ss : T ⊆ U) : s ⊧ₛ* T :=
+  fun _ hf => h (ss hf)
+
+@[simp] lemma modelsTheoryEmpty {s : Struc M} : s ⊧ₛ* (∅ : Set F) := fun p => by simp
+
+@[simp] lemma modelsTheory_insert {T : Set F} {f : F} {s : Struc M} :
+    s ⊧ₛ* insert f T ↔ s ⊧ₛ f ∧ s ⊧ₛ* T := by
+  simp[modelsTheory]
+
+@[simp] lemma modelsTheory_union {T U : Set F} {s : Struc M} :
+    s ⊧ₛ* T ∪ U ↔ s ⊧ₛ* T ∧ s ⊧ₛ* U := by
+  simp[modelsTheory]
+  exact
+  ⟨fun h => ⟨fun f hf => h (Or.inl hf), fun f hf => h (Or.inr hf)⟩,
+   by rintro ⟨h₁, h₂⟩ f (h | h); exact h₁ h; exact h₂ h⟩
+
+@[simp] lemma modelsTheory_image {f : α → F} {A : Set α} {s : Struc M} :
+    s ⊧ₛ* f '' A ↔ ∀ i ∈ A, s ⊧ₛ (f i) := by simp[modelsTheory]
+
+@[simp] lemma modelsTheory_range {f : α → F} {s : Struc M} :
+    s ⊧ₛ* Set.range f ↔ ∀ i, s ⊧ₛ (f i) := by simp[modelsTheory]
+
+lemma satisfiableₛ_of_subset {T U : Set F} (h : Satisfiableₛ U) (ss : T ⊆ U) : Satisfiableₛ T :=
+  by rcases h with ⟨M, i, s, h⟩; exact ⟨M, i, s, modelsTheory_of_subset h ss⟩
+
+lemma consequence_iff {T : Set F} {f : F} : T ⊨ f ↔ ¬Satisfiableₛ (insert (~f) T) := by
+  simp[consequence, Satisfiableₛ]; constructor
+  · intro h M hM s hf hT; have : s ⊧ₛ f := h M s hT; contradiction
+  · intro h M hM s; contrapose; exact h M hM s
+
+end Semantics
+
+variable (F)
+variable [LogicSymbol F] {Struc : Type w → Type v} [𝓢 : Semantics F Struc]
+
+class Compact where
+  compact {T : Set F} : Semantics.Satisfiableₛ T ↔ (∀ u : Finset F, (u : Set F) ⊆ T → Semantics.Satisfiableₛ (u : Set F))
+
+variable {F}
+
+namespace Compact
+
+variable [Compact F]
+variable {M : Type w} [Inhabited M] {s : Struc M}
+
+lemma conseq_compact [DecidableEq F] {f : F} :
+    T ⊨ f ↔ ∃ u : Finset F, ↑u ⊆ T ∧ u ⊨ f := by
+  simp[Semantics.consequence_iff, compact (T := insert (~f) T)]
+  constructor
+  · intro ⟨u, ss, hu⟩; exact ⟨Finset.erase u (~f), by simp[ss], by { simp; intro h; exact hu (Semantics.satisfiableₛ_of_subset h (by simp)) }⟩
+  · intro ⟨u, ss, hu⟩; exact ⟨insert (~f) u, by simpa using Set.insert_subset_insert ss, by simpa using hu⟩
+
+end Compact
+
+end LO
